theories/Syntax/UntypedReduction.v
@@ -8,11 +8,57 @@ From LogRel.Syntax Require Import BasicAst Context NormalForms (* Weakening *) C
 
 (** *** One-step reduction. *)
 
+Fixpoint whns_all {red : term -> term -> Type} (Pred : forall t t', red t t' -> Type)
+  {k v t} (w : @whns red k v t) {struct w} : Type :=
+  match w with
+  | whns_tEval notink => unit
+  | whns_tApp w => whns_all Pred w
+  | whns_tNatElim w => whns_all Pred w
+  | whns_tBoolElim w => whns_all Pred w
+  | whns_tEmptyElim w => whns_all Pred w
+  | whns_tTreeElim w => whns_all Pred w
+  | whns_tFst w => whns_all Pred w
+  | whns_tSnd w => whns_all Pred w
+  | whns_tIdElim w => whns_all Pred w
+  | whns_tAlpha w => whns_all Pred w
+  | whns_tXi w => whns_all Pred w
+  | whns_tXXi w => whns_all Pred w
+  | whns_tXXiRed w notink' r w'=> whns_all Pred w × Pred _ _ r × whns_all Pred w'
+  end.
+
+Fixpoint whns_all_forall red Pred : (forall t t' (r : red t t'), Pred _ _ r) ->
+  forall k v t (w : @whns red k v t), whns_all Pred w.
+Proof.
+  intros allr k v t w.
+  destruct w.
+  2-12: cbn; eapply whns_all_forall, allr.
+  + constructor.
+  + repeat constructor.
+    - eapply whns_all_forall, allr.
+    - eapply allr.
+    - eapply whns_all_forall, allr.
+Defined.
 
 
 Inductive closure (R : term -> term -> Type) : term -> term -> Type :=
   | clos_nil t : closure R t t
   | clos_cons t t' u : closure R t' u -> R t t' -> closure R t u.
+
+Fixpoint closure_all {R : term -> term -> Type} (PR : forall t t', R t t' -> Type)
+  {t t'} (rtt' : closure R t t') {struct rtt'} : Type :=
+  match rtt' with
+  | clos_nil _ t => unit
+  | clos_cons _ t t' u rt'u rtt' => closure_all PR rt'u × PR _ _ rtt'
+  end.
+
+Fixpoint closure_all_forall R PR : (forall t t' (rtt' : R t t'), PR _ _ rtt') -> forall t t' (rtt' : closure R t t'), closure_all PR rtt'.
+Proof.
+  intros allr t t' rtt'.
+  destruct rtt'; constructor.
+  - eapply closure_all_forall, allr.
+  - eapply allr.
+Defined.
+
 
 
 Inductive OneRedAlg {L : list ell} : term -> term -> Type :=
@@ -71,12 +117,89 @@ Inductive OneRedAlg {L : list ell} : term -> term -> Type :=
 | evalRel v k b (ℓ : ell) : in_ell ℓ k b ->
   [ L |tApp (tEval ℓ (tRel v)) (nat_to_term k) ⤳ (bool_to_term b) ]
 | evalBox ℓ ℓ' t : [ L | tEval ℓ (tBox ℓ' t) ⤳ t]
-| xiSubst ℓ n n': [L | n ⤳ n'] -> [L | tXi ℓ n ⤳ tXi ℓ n']
+| xiSubst ℓ n n' k : [L | n ⤳ n'] -> [L | tXi ℓ (nSucc k n) ⤳ tXi ℓ (nSucc k n')]
 | xiLeaf ℓ n : [L | tXi ℓ (nat_to_term n) ⤳ tLeaf (nat_to_term n) ]
-| xiNode (ℓ : ell) n (k : newnat ℓ) : whns (red := closure OneRedAlg) 0 k n ->
+| xiNode (ℓ : ell) n (k : newnat ℓ) : whns (red := closure OneRedAlg) k 0 n ->
   [L |tXi ℓ n ⤳ tNode (nat_to_term k) (tXi (cons_ell ℓ k true) n) (tXi (cons_ell ℓ k false) n) ]
+| xxiSubst ℓ m m' n k : [L | m ⤳ m'] -> [L | tXXi ℓ (nSucc k m) n ⤳ tXXi ℓ (nSucc k m') n]
 
 where "[ L | t ⤳ t' ]" := (@OneRedAlg L t t') : typing_scope.
+
+Fixpoint OneRedAlg_rect_with_all
+  (L : list ell) (P : forall t t0 : term, [L | t ⤳ t0] -> Type)
+  (hBRed : forall A a t : term, P (tApp (tLambda A t) a) t[a..] BRed)
+  (happSubst : forall (t u a : term) (o : [L | t ⤳ u]), P t u o -> P (tApp t a) (tApp u a) (appSubst o))
+  (hnatElimSubst : forall (P0 hz hs n n' : term) (o : [L | n ⤳ n']),
+   P n n' o -> P (tNatElim P0 hz hs n) (tNatElim P0 hz hs n') (natElimSubst o))
+  (hnatElimZero : forall P0 hz hs : term, P (tNatElim P0 hz hs tZero) hz natElimZero)
+  (hnatElimSucc : forall P0 hz hs n : term,
+   P (tNatElim P0 hz hs (tSucc n)) (tApp (tApp hs n) (tNatElim P0 hz hs n)) natElimSucc)
+  (hboolElimSubst : forall (P0 ht hf n n' : term) (o : [L | n ⤳ n']),
+   P n n' o -> P (tBoolElim P0 ht hf n) (tBoolElim P0 ht hf n') (boolElimSubst o))
+  (hboolElimTrue : forall P0 ht hf : term, P (tBoolElim P0 ht hf tTrue) ht boolElimTrue)
+  (hboolElimFalse : forall P0 ht hf : term, P (tBoolElim P0 ht hf tFalse) hf boolElimFalse)
+  (halphaSubst : forall (i k : nat) (n n' : term) (o : [L | n ⤳ n']),
+   P n n' o -> P (tApp (tAlpha i) (nSucc k n)) (tApp (tAlpha i) (nSucc k n')) (alphaSubst o))
+  (halphaRed : forall (i : list_index L) (n : nat) (b : bool) (hin : in_ell (list_at L i) n b),
+   P (tApp (tAlpha i) (nat_to_term n)) (bool_to_term b) (alphaRed hin))
+  (hemptyElimSubst : forall (P0 e e' : term) (o : [L | e ⤳ e']),
+   P e e' o -> P (tEmptyElim P0 e) (tEmptyElim P0 e') (emptyElimSubst o))
+  (htreeElimSubst : forall (P0 hl hn t t' : term) (o : [L | t ⤳ t']),
+   P t t' o -> P (tTreeElim P0 hl hn t) (tTreeElim P0 hl hn t') (treeElimSubst o))
+  (htreeElimLeaf : forall P0 hl hn n : term, P (tTreeElim P0 hl hn (tLeaf n)) (tApp hl n) treeElimLeaf)
+  (htreeElimNode : forall P0 hl hn n tl tr : term,
+   P (tTreeElim P0 hl hn (tNode n tl tr))
+     (tApp (tApp (tApp (tApp (tApp hn n) tl) tr) (tTreeElim P0 hl hn tl)) (tTreeElim P0 hl hn tr))
+     treeElimNode)
+  (hfstSubst : forall (p p' : term) (o : [L | p ⤳ p']), P p p' o -> P (tFst p) (tFst p') (fstSubst o))
+  (hfstPair : forall A B a b : term, P (tFst (tPair A B a b)) a fstPair)
+  (hsndSubst : forall (p p' : term) (o : [L | p ⤳ p']), P p p' o -> P (tSnd p) (tSnd p') (sndSubst o))
+  (hsndPair : forall A B a b : term, P (tSnd (tPair A B a b)) b sndPair)
+  (hidElimRefl : forall A x P0 hr y A' z : term, P (tIdElim A x P0 hr y (tRefl A' z)) hr idElimRefl)
+  (hidElimSubst : forall (A x P0 hr y e e' : term) (o : [L | e ⤳ e']),
+   P e e' o -> P (tIdElim A x P0 hr y e) (tIdElim A x P0 hr y e') (idElimSubst o))
+  (hevalRel : forall (v k : nat) (b : bool) (ℓ : ell) (i : in_ell ℓ k b),
+   P (tApp (tEval ℓ (tRel v)) (nat_to_term k)) (bool_to_term b) (evalRel v k b ℓ i))
+  (hevalBox : forall (ℓ ℓ' : ell) (t : term), P (tEval ℓ (tBox ℓ' t)) t (evalBox ℓ ℓ' t))
+  (hxiSubst : forall (ℓ : ell) (n n' : term) k (o : [L | n ⤳ n']),
+   P n n' o -> P (tXi ℓ (nSucc k n)) (tXi ℓ (nSucc k n')) (xiSubst ℓ n n' k o))
+  (hxiLeaf : forall (ℓ : ell) (n : nat), P (tXi ℓ (nat_to_term n)) (tLeaf (nat_to_term n)) (xiLeaf ℓ n))
+  (hxiNode : forall (ℓ : ell) (n : term) (k : newnat ℓ) (w : whns k 0 n), whns_all (fun t t' => closure_all P) w ->
+   P (tXi ℓ n) (tNode (nat_to_term k) (tXi (cons_ell ℓ k true) n) (tXi (cons_ell ℓ k false) n))
+     (xiNode ℓ n k w))
+  (hxxiSubst : forall (ℓ : ell) (m m' n : term) (k : nat) (o : [L | m ⤳ m']), P m m' o ->
+   P (tXXi ℓ (nSucc k m) n) (tXXi ℓ (nSucc k m') n) (xxiSubst ℓ m m' n k o))
+  (t t0 : term) (o : [L | t ⤳ t0]) {struct o}: P t t0 o.
+Proof.
+  destruct o.
+  + eapply hBRed.
+  + eapply happSubst, OneRedAlg_rect_with_all; tea.
+  + eapply hnatElimSubst, OneRedAlg_rect_with_all; tea.
+  + eapply hnatElimZero.
+  + eapply hnatElimSucc.
+  + eapply hboolElimSubst, OneRedAlg_rect_with_all; tea.
+  + eapply hboolElimTrue.
+  + eapply hboolElimFalse.
+  + eapply halphaSubst, OneRedAlg_rect_with_all; tea.
+  + eapply halphaRed.
+  + eapply hemptyElimSubst, OneRedAlg_rect_with_all; tea.
+  + eapply htreeElimSubst, OneRedAlg_rect_with_all; tea.
+  + eapply htreeElimLeaf.
+  + eapply htreeElimNode.
+  + eapply hfstSubst, OneRedAlg_rect_with_all; tea.
+  + eapply hfstPair.
+  + eapply hsndSubst, OneRedAlg_rect_with_all; tea.
+  + eapply hsndPair.
+  + eapply hidElimRefl.
+  + eapply hidElimSubst, OneRedAlg_rect_with_all; tea.
+  + eapply hevalRel.
+  + eapply hevalBox.
+  + eapply hxiSubst, OneRedAlg_rect_with_all; tea.
+  + eapply hxiLeaf.
+  + eapply hxiNode, whns_all_forall, closure_all_forall, OneRedAlg_rect_with_all; tea.
+  + eapply hxxiSubst, OneRedAlg_rect_with_all; tea.
+Qed.
+
 
 (* Keep in sync with OneRedTermDecl! *)
 
@@ -119,13 +242,6 @@ Record cored L t t' : Prop := { _ : [L |t' ⤳ t] }.
 Ltac inv_whne :=
   match goal with [ H : whne _ |- _ ] => inversion H end.
 
-Lemma nSucc_nat_to_term t n k : nat_to_term n = nSucc k t -> exists k', nat_to_term k' = t.
-Proof.
-  induction k in n |-*.
-  + now exists n.
-  + destruct n; inversion 1.
-    now eapply IHk.
-Qed.
 
 Lemma whne_nored {L} n u :
   @whne (@RedClosureAlg L) n -> [ L | n ⤳ u] -> False.
@@ -141,9 +257,10 @@ Proof.
     - inversion ne.
   * eapply nSucc_nat_to_term in H1 as [[] <-];
     inversion ne.
-  * destruct k.
+  * eapply nSucc_eq_inv in H1 as [[<- <-]| [(?&->&<-)|(?&<-&->)]].
     - easy.
     - inversion X.
+    - inversion ne.
   * eapply nSucc_nat_to_term in H1 as [[] <-];
     inversion ne.
   * destruct k.
@@ -155,7 +272,7 @@ Ltac inv_alpha :=
   match goal with
     [ H : [_ | tAlpha _ ⤳ _] |- _ ] => inversion H
     | [ H : whne (tAlpha _) |- _ ] => inversion H end.
-Lemma whnf_nored L n u :
+(* Lemma whnf_nored L n u :
   @whnf (@RedClosureAlg L) n -> [ L | n ⤳ u] -> False.
 Proof.
   intros nf red.
@@ -164,107 +281,202 @@ Proof.
   now eapply whne_nored.
   admit.
 Admitted.
-
+ *)
 (** *** Determinism of reduction *)
 
 Lemma ored_detaux : forall {L i i' n n'}, [ L | tApp (tAlpha i) (nat_to_term n) ⤳ tApp (tAlpha i') n'] -> False.
 Proof.
   intros L i i' n n' H.
   inversion H; subst; clear H.
-  * inversion H1.
-  * induction k in n0, n, H1, H2 |-*; cbn in H2.
-    - rewrite -> H2 in H1.
-      destruct n; inversion H1.
-    - destruct n; inversion H2.
-      now eapply IHk.
+  * inversion X.
+  * eapply eq_sym, nSucc_nat_to_term in H2 as [[] <-].
+    - inversion X.
+    - inversion X.
   * destruct b; inversion H3.
 Qed.
 
-Lemma ored_det {L t u v} :
-  [L | t ⤳ u] -> [L | t ⤳ v] ->
-  u = v.
+#[local] Ltac nSucc_handler :=
+try match goal with
+| eq : nSucc ?k ?t = nSucc ?k' ?t' |- _ =>
+    eapply nSucc_eq_inv in eq as [[<- <-] | [(?&->&<-)|(?&<-&->)]]
+| eq : nSucc ?k ?t  = nat_to_term ?k' |- _ =>
+    eapply symmetry, nSucc_nat_to_term in eq as [[] <-]
+| eq : nat_to_term ?k = nSucc ?k' ?t' |- _ =>
+    eapply nSucc_nat_to_term in eq as [[] <-]
+| eq  : nat_to_term ?k =  nat_to_term ?k' |- _ =>
+    eapply nat_to_term_inj in eq as <-
+end.
+
+(* Lemma det_closure L t n k v (r : [ L | t ⤳* n ]) : @whns (@RedClosureAlg L) k v n ->
+  closure_all (fun t u _ => (forall v, [L | t ⤳ v] -> u = v) /\
+    (forall k v : nat, @whns (@RedClosureAlg L) k v t -> False)) r ->
+    forall n' k' v', @whns (@RedClosureAlg L) k' v' n' ->[L | t ⤳* n' ] -> n = n'.
 Proof.
-  intros red red'.
-  induction red in v, red' |- *.
-  - inversion red' ; subst ; clear red'.
-    + reflexivity.
-    + exfalso.
-      eapply whnf_nored, H2.
-      now econstructor.
-  - inversion red' ; subst ; clear red'; try inv_alpha.
-    + exfalso.
-      eapply whnf_nored, red.
-      now econstructor.
-    + f_equal.
-      eauto.
-    + inversion red.
-  - inversion red'; subst.
-    2,3: exfalso; eapply whnf_nored; tea; constructor.
-    f_equal; eauto.
-  - inversion red'; try reflexivity; subst.
-    exfalso; eapply whnf_nored; tea; constructor.
-  - inversion red'; try reflexivity; subst.
-    exfalso; eapply whnf_nored; tea; constructor.
-  - inversion red'; subst.
-    2,3: exfalso; eapply whnf_nored; tea; constructor.
-    f_equal; eauto.
-  - inversion red'; try reflexivity; subst.
-    exfalso; eapply whnf_nored; tea; constructor.
-  - inversion red'; try reflexivity; subst.
-    exfalso; eapply whnf_nored; tea; constructor.
-  - inversion red'; subst.
-    + inv_alpha.
-    + f_equal.
-      eapply nSucc_eq_inv in H1 as [[<- <-]| [(m'&->&<-)|(m&<-&->)]].
-      * now f_equal.
-      * inversion H2.
-      * inversion red.
-    + eapply nSucc_nat_to_term in H1 as [[] <-];
-      inversion red.
-  - inversion red'; subst.
-    + inv_alpha.
-    + symmetry in H1;
-      eapply nSucc_nat_to_term in H1 as [[] <-];
-      inversion H2.
-    + eapply nat_to_term_inj in H1 as <-.
-      eapply index_to_nat_inj in H0 as <-.
-      f_equal. now eapply functionality; constructor.
-  - inversion red'; subst.
-    f_equal; eauto.
-  - inversion red'; subst.
-    2,3: exfalso; eapply whnf_nored; tea; constructor.
-    f_equal; eauto.
-  - inversion red'; try reflexivity; subst.
-    exfalso; eapply whnf_nored; tea; constructor.
-  - inversion red'; try reflexivity; subst.
-    exfalso; eapply whnf_nored; tea; constructor.
-  - inversion red'; subst; clear red'.
-    1: f_equal; now eapply IHred.
-    exfalso; eapply whnf_nored; tea; constructor.
-  - inversion red'; subst; try reflexivity.
-    exfalso; eapply whnf_nored; tea; constructor.
-  - inversion red'; subst; clear red'.
-    1: f_equal; now eapply IHred.
-    exfalso; eapply whnf_nored; tea; constructor.
-  - inversion red'; subst; try reflexivity.
-    exfalso; eapply whnf_nored; tea; constructor.
-  - inversion red'; subst; try reflexivity.
-    exfalso; eapply whnf_nored;tea; constructor.
-  - inversion red'; subst.
-    2: f_equal; eauto.
-    exfalso; eapply whnf_nored;tea; constructor.
-  - inversion red'; subst.
-    + inversion H2.
-    + eapply nat_to_term_inj in H2 as <-.
-      f_equal. now eapply functionality; constructor.
-  - now inversion red'; subst.
-  - inversion red'; subst; clear red'.
-    + now f_equal.
-    + destruct n0; inversion red.
-  - inversion red'; subst.
-    + destruct n; inversion H2.
-    + reflexivity.
+  intros w allr ??? w' r'.
+  induction r; inversion r'; subst; clear r'.
+  + reflexivity.
+  + cbn in allr. *)
+Goal forall L t, (forall u, [L | t ⤳ u] -> forall k v, @whns (@RedClosureAlg L) k v t -> False) ->
+  (forall u, [L | t ⤳* u] -> forall k v, @whns (@RedClosureAlg L) k v t -> t = u).
+Proof.
+  intros.
+  induction X.
+  reflexivity.
+  exfalso; eauto.
 Qed.
+
+(* Lemma wk_det L t n (r : [L | t ⤳* n]) :
+  (forall u, [L | t ⤳* u] ->forall k v, @whns (@RedClosureAlg L) k v t -> t = u) ->
+  closure_all (fun t u _ => (forall v, [L | t ⤳ v] -> u = v) /\
+    (forall k v : nat, @whns (@RedClosureAlg L) k v t -> False)) r ->
+  closure_all (fun t _ _ =>
+    forall u, [L | t ⤳* u] ->forall k v, @whns (@RedClosureAlg L) k v t -> t = u) r.
+Proof.
+  intros.
+  induction r.
+  + cbn in *. constructor.
+  + constructor.
+    - eapply IHr; clear IHr.
+      * cbn in X.
+        destruct r.
+       ++ cbn in *.
+          intros. *)
+
+Definition instant_det {L} t u (r : [L | t ⤳ u]) := (forall u', [L | t ⤳ u'] -> u = u')
+  /\ (forall k v, @whns (closure (@OneRedAlg L)) k v t -> False).
+
+
+
+Lemma whs_det L t n (r : [L | t ⤳* n]) :
+  (forall u (r : [L | n ⤳ u]), instant_det n u r) ->
+  closure_all (instant_det (L:=L)) r ->
+  forall k v, @whns (@RedClosureAlg L) k v n ->
+  forall n', [L | t ⤳* n'] ->
+  forall k' v', @whns (@RedClosureAlg L) k' v' n' ->
+  n = n'.
+Proof.
+  intros tdet allr ?? w ? r' ?? w'.
+  induction r; inversion r'; subst; clear r'.
+  + reflexivity.
+  + exfalso.
+    specialize (tdet _ X0) as []. eauto.
+  + destruct allr as (allr&hred&hwhns).
+    exfalso. eauto.
+  + destruct allr as (allr&hred&hwhns).
+    eapply IHr; tea.
+    now destruct (hred _ X0).
+Qed.
+
+
+Lemma whns_uniq_k L k v t (w : @whns (closure (@OneRedAlg L)) k v t) :
+  whns_all (fun _ _ => closure_all (instant_det (L:=L))) w ->
+  forall k', @whns (closure (@OneRedAlg L)) k' v t -> k = k'.
+Proof.
+(*   intros allw ? w'.
+  induction w' in k, w, allw |-*; revert allw; dependent inversion w; subst; cbn; clear w; intros ?; nSucc_handler; eauto.
+  all : try solve [inversion w'| inversion w0].
+  + admit.
+  + admit.
+  + inversion w'1.
+  + destruct (IHw'1 _ w0 ltac:(eapply allw)).
+    
+    eapply IHw'2.
+   destruct allw; eapply IHw'; tea. specialize (IHw' _ _ _ allw) as [<- ev].
+    now inversion ev.
+  + specialize (IHw' _ _ _ allw) as [<- ev].
+    now inversion ev.
+  + destruct allw as (allw1&hr&allw2).
+    specialize (IHw' _ _ _ allw1) as [<- ev].
+    now inversion ev.
+  + specialize (IHw'1 _ _ _ allw) as [<- ev].
+    now inversion ev.
+  + inversion w'1.
+  + destruct allw as (allw0&allc&allw1).
+    assert (forall t' (r : [L | n' ⤳ t']), instant_det n' t' r).
+    { intros.
+      split.
+      - intros. *)
+Admitted.
+
+
+Lemma whns_uniq_kv L k v t (w : @whns (closure (@OneRedAlg L)) k v t) :
+  whns_all (fun _ _ => closure_all (instant_det (L:=L))) w ->
+  forall k' v', @whns (closure (@OneRedAlg L)) k' v' t -> k = k' /\ v = v'.
+Proof.
+  intros allw ?? w'.
+  induction w' in k, v, w, allw |-*; revert allw; dependent inversion w; subst; cbn; clear w; intros ?; nSucc_handler; eauto.
+  all : try solve [inversion w'| inversion w0].
+  + specialize (IHw' _ _ _ allw) as [<- ev].
+    now inversion ev.
+  + specialize (IHw' _ _ _ allw) as [<- ev].
+    now inversion ev.
+  + destruct allw as (allw1&hr&allw2).
+    specialize (IHw' _ _ _ allw1) as [<- ev].
+    now inversion ev.
+  + specialize (IHw'1 _ _ _ allw) as [<- ev].
+    now inversion ev.
+  + inversion w'1.
+  + destruct allw as (allw0&allc&allw1).
+    assert (forall t' (r : [L | n' ⤳ t']), instant_det n' t' r).
+    { intros.
+      split.
+      - intros.
+
+Admitted.
+
+Lemma ored_no_whns {L t u} :
+  [L | t ⤳ u] -> forall k v, @whns (@RedClosureAlg L) k v t -> False.
+Proof.
+  intros red k v w.
+  induction red using OneRedAlg_rect_with_all in k, v, w |-*;
+    inversion w; subst; clear w; nSucc_handler; eauto.
+  all: try solve [inversion X |inversion red].
+  * destruct (notin_is_not_in ltac:(tea) ltac:(tea)).
+  * destruct k'.
+    2: inversion w0.
+    cbn in w0.
+    admit.
+Admitted.
+
+Lemma ored_det {L t u} :
+  [L | t ⤳ u] -> (forall v, [L | t ⤳ v] ->
+  u = v) /\ (forall k v, @whns (@RedClosureAlg L) k v t -> False).
+Proof.
+  intros red.
+  induction red using OneRedAlg_rect_with_all; try destruct IHred as [IHredred IHredwhns].
+  1-26 : split;
+    [intros t_r red'; inversion red'; subst; clear red'; nSucc_handler; repeat f_equal; eauto
+    |intros k_w v_w wt; inversion wt; subst; clear wt; nSucc_handler; eauto]; try solve [inversion X | inversion red].
+  * eapply index_to_nat_inj in H0 as <-.
+    eapply functionality; tea.
+  * eapply functionality; tea.
+  * destruct (notin_is_not_in H0 i).
+  * destruct k.
+    2: inversion X.
+    destruct (IHredwhns _ _ X).
+  * destruct n; inversion X.
+  * destruct k0.
+    2: inversion w.
+    exfalso; cbn in *.
+    induction w in X, n', X0 |-* ; inversion X0; subst; clear X0; nSucc_handler.
+    all: try solve [inversion X1 | inversion w | eapply IHw; tea].
+    + destruct (notin_is_not_in n H3).
+    + destruct k'.
+      2: inversion X1.
+      cbn in *.
+      specialize (IHw X).
+      admit.
+    + destruct X as (?&?&?).
+      eapply IHw1; tea.
+    + inversion w1.
+  * destruct n0; inversion w.
+  * admit.
+  * admit.
+  * admit.
+  * destruct k'.
+    2: inversion w.
+    cbn in w.
+Admitted.
 
 Lemma red_whne {L} t u : [ L | t ⤳* u] -> whne t -> t = u.
 Proof.
